Types.v
@@ -13,22 +13,30 @@ Delimit Scope reft_scope with reft.
 
 (** Type Language **)
 Inductive base_type : Set :=
-  | int_t  : base_type.
+  | int_t  : base_type
+  | null_t : base_type
+  | ref_t : loc -> base_type.
 
 Definition base_of_type b :=
   match b with
     | int_t => nat
+    | null_t => unit
+    | ref_t l => loc
   end.
 
 Definition base_of_val (v: value) :=
   match v with
     | int_v  _ => int_t
+    | loc_v  l => ref_t l
+    | null     => null_t
   end.
 
 Definition val_of_base : forall (b : base_type), (base_of_type b) -> value :=
   fun b => 
     match b with
       | int_t => fun x => int_v x
+      | ref_t l => fun _ => loc_v l
+      | null_t => fun _ => null
     end.
 
 Inductive brel : Set :=
@@ -79,6 +87,17 @@ Definition subst_r_var (s : subst_t var var) reft :=
   mkReft_type (reft_base reft)
               (subst s (reft_r reft)).
 
+Definition subst_base_loc (s : subst_t loc loc) b :=
+  match b with
+    | ref_t l => ref_t (s l)
+    | _ => b
+  end.
+
+Instance Subst_base_loc : Subst base_type loc loc := subst_base_loc.
+
+Definition subst_r_loc (s : subst_t loc loc) reft :=
+  mkReft_type (subst s (reft_base reft)) (reft_r reft).
+
 Definition subst_r s reft :=
   mkReft_type (reft_base reft)
               (subst s (reft_r reft)).
@@ -88,20 +107,6 @@ Instance Subst_reft : Subst reft_type var expr := subst_r.
 
 Definition type_binding : Set := (var * reft_type)%type.
 
-Record proc_schema : Set :=
-  mkSchema { s_formals: list var;
-             s_formal_ts: list reft_type;
-             s_ret: type_binding }.
-
-Definition subst_schema s S :=
-  let subst_both s xt := (subst s (fst xt), subst s (snd xt)) in
-  match S with
-    | mkSchema xs ts xt =>
-      mkSchema (subst s xs) (subst s ts) (subst_both s xt)
-  end.
-
-Instance Subst_proc_schema : Subst proc_schema var var := subst_schema.
-
 Definition dummyt (v : var) t p := mkReft_type t p.
 
 Notation "x .= y" := (rel_r x eq_brel y) (at level 70).
@@ -110,8 +115,29 @@ Notation "{ vv : t | P }" := (dummyt vv t P%reft) (at level 0, vv at level 99, n
 
 
 (** Environments **)
-Definition bind_env (B T : Type) := list (B * T)%type.
-Definition type_env : Type := bind_env var reft_type.
+Definition bind_env (B T : Set) : Set := list (B * T)%type.
+Definition type_env : Set := bind_env var reft_type.
+Definition heap_env : Set := bind_env loc (var * reft_type)%type.
+
+(** Procedures **)
+Record proc_schema : Set :=
+  mkSchema { s_formals: list var;
+             s_formal_ts: list reft_type;
+             s_heap_in: heap_env;
+             s_heap_out: heap_env;
+             s_ret: type_binding }.
+
+Definition subst_schema (s S :=
+  let subst_both s xt := (subst s (fst xt), subst s (snd xt)) in
+  match S with
+    | mkSchema xs ts hi ho xt =>
+      mkSchema (subst s xs) (subst s ts) (subst s hi) (subst s ho) (subst_both s xt)
+  end.
+
+Definition 
+
+Instance Subst_proc_schema : Subst proc_schema var var := subst_schema.
+
 Definition proc_env : Type := bind_env pname (stmt * proc_schema)%type.
 
 Definition var_in : var -> type_env -> Prop := 
@@ -119,6 +145,18 @@ Definition var_in : var -> type_env -> Prop :=
 
 Definition var_not_in : var -> type_env -> Prop :=
   fun x Γ => Forall (fun xt => (fst xt <> x)) Γ.
+
+Definition bind_in : var -> heap_env -> Prop :=
+  fun x Σ => exists l t, In (l, (x, t)) Σ.
+
+Definition bind_not_in : var -> heap_env -> Prop :=
+  fun x Σ => Forall (fun lxt => (fst (snd lxt)) <> x) Σ.
+
+Definition loc_in : loc -> heap_env -> Prop :=
+  fun l Σ => exists b, In (l, b) Σ.
+
+Definition loc_not_in : loc -> heap_env -> Prop :=
+  fun l Σ => Forall (fun lxt => (fst lxt <> l)) Σ.
 
 Definition fun_in : (pname * (stmt * proc_schema)) -> proc_env -> Prop :=
   fun ft Φ => In ft Φ.
@@ -139,7 +177,7 @@ Definition guards := list reft_prop.
 (** Ugh Equality **)
 Instance EqDec_base_t : EqDec base_type := _.
 Proof.
-  hnf. decide equality.
+  hnf. decide equality; apply eq_dec.
 Qed.
 
 Instance EqDec_brel_t : EqDec brel := _.
