TranslationLemmas.v
@@ -1,1 +1,1286 @@
+Add LoadPath "vst".
+Require Import msl.Coqlib2.
+Require Import msl.log_normalize.
+Require Import msl.eq_dec.
+Require Import Coq.Unicode.Utf8.
+Require Import Coq.Program.Equality.
+
+Require Import Types.
+Require Import Judge.
+Require Import Subst.
+Require Import ProgramLogic.
+Require Import Translation.
+Require Import Language.
+Require Import WFLemmas.
+Require Import SubstLemmas.
+Require Import EvalLemmas.
+Require Import Tactics.
+Require Import List.
+Import ListNotations.
+
+Lemma forall_p_combine :
+  forall (X Y : Type) (P : Y -> Prop) (xs : list X) (ys : list Y),
+    length xs = length ys ->
+    Forall P ys -> 
+    Forall (fun xy => P (snd xy)) (combine xs ys).
+Proof.
+  intros.
+  rewrite Forall_forall in *.
+  intros.
+  destruct x as [x y].
+  simpl in *.
+  pose (combine_split xs ys H).
+  specialize (H0 y).
+  apply in_combine_r in H1.
+  apply H0.
+  assumption.
+Qed.
+
+Lemma sub_eq_expr :
+  forall (e : expr) x x', 
+    subst (subst_one x (var_e x')) e 
+    = subst (fun i => if eq_dec i x then x' else i) e.
+Proof.
+  induction e.
+  * reflexivity.
+  * intros. unfold subst. simpl. unfold subst_one. foo. 
+  * intros.
+    unfold subst at 1.
+    unfold Subst_var_expr.
+    unfold Language.subst_expr.
+    rewrite IHe1.
+    rewrite IHe2.
+    reflexivity.
+Qed.
+  
+Lemma sub_eq :
+  forall (p : reft_prop) x x', 
+    subst (subst_one x (var_e x')) p 
+    = subst (fun i => if eq_dec i x then x' else i) p.
+Proof.
+  intros.
+  induction p.
+  constructor.
+  unfold subst.
+  unfold Subst_prop, Subst_prop_var, subst_prop, subst_prop_var.
+  rewrite sub_eq_expr.
+  rewrite sub_eq_expr.
+  reflexivity.
+  unfold subst in *.
+  simpl.
+  rewrite IHp.
+  reflexivity.
+  unfold subst in *.
+  simpl.
+  rewrite IHp1.
+  rewrite IHp2.
+  reflexivity.
+  unfold subst in *.
+  simpl.
+  rewrite IHp1.
+  rewrite IHp2.
+  reflexivity.
+Qed.
+
+Lemma subst_vv_ty:
+  forall x x' T,
+    x <> ν ->
+    sep_ty (var_e x) T 
+    |-- subst (subst_one ν x') (sep_ty (var_e x) T).
+Proof.
+  intros.
+  unfold subst.
+  unfold sep_ty.
+  destruct T as [b p].
+  rewrite subst_distr_andp.
+  apply andp_derives.
+  rewrite subst_distr_andp.
+  apply andp_derives.
+  unfold sep_base.
+  unfold subst, Subst_pred, subst_pred.
+  simpl in *.
+  intro w.
+  apply exp_left.
+  intro vv.
+  rewrite <- exp_andp1.
+  apply andp_derives.
+  normalize.
+  apply (exp_right vv).
+  apply prop_right.
+  unfold subst_one. 
+  destruct (eq_dec x ν).
+    congruence.
+    rewrite <- H0. reflexivity.
+  apply derives_refl.
+  intro w.
+  unfold subst at 2, Subst_pred, subst_pred.
+  repeat rewrite <- subst_ty_prop.
+  unfold subst, Subst_pred, subst_pred.
+  assert
+     ((λ i : var, eval w (subst_one ν (var_e x) i))
+      = (λ i : var,
+               eval (fun i0 => eval w (subst_one ν x' i0), hp w)
+                    (subst_one ν (var_e x) i))).
+  extensionality i.
+  unfold subst_one. 
+  destruct (eq_dec i ν). 
+  simpl.
+  destruct (eq_dec x ν). intuition. reflexivity.
+  destruct (eq_dec i ν). intuition. simpl.
+  destruct (eq_dec i ν). intuition. reflexivity.
+  rewrite <- H0.
+  simpl.
+  apply derives_refl.
+  normalize.
+Qed.
+ 
+Lemma vv_sub_env :
+  forall G,  
+    var_not_in ν G -> 
+      (forall x,
+         sep_env G |-- subst (subst_one ν x) (sep_env G)).
+Proof.
+  intro G.
+  induction G.
+  + simpl. trivial.
+  + destruct a as [b p].
+    unfold sep_env in *.
+    fold sep_env in *.
+    intro H.
+    intro e.
+    repeat rewrite subst_distr_andp.
+    apply andp_derives.
+    apply andp_derives.
+    apply subst_vv_ty.
+    unfold var_not_in in H.
+    rewrite Forall_forall in H.
+    apply H with (x := (b, p)).
+    left. reflexivity.
+    apply IHG.
+    inversion H.
+    assumption.
+    trivial.
+Qed.
+
+Lemma vv_sub_guards :
+  forall G Grds,
+    wf_guards G Grds -> 
+      forall (x : expr),
+      sep_guards Grds |-- subst (subst_one ν x) (sep_guards Grds).
+Proof.
+  intros G Grds.
+  induction Grds as [| p].
+  + simpl. trivial.
+  + intros wf x.
+    unfold sep_guards in *; fold sep_guards in *.
+    inversion wf. subst.
+    pose (wf_guards_vv_nonfree G Grds H2).
+    repeat rewrite subst_distr_andp.
+    repeat apply andp_derives.
+    rewrite subst_nonfree_prop.
+    apply derives_refl.
+    apply H1.
+    apply n.
+    trivial.
+Qed.
+
+Lemma subtype_interp_pred :
+  forall Γ Ξ φ φ' x b,
+    var_not_in ν Γ ->
+    wf_guards Γ Ξ -> 
+    subtype Γ Ξ { ν : b | φ } { ν : b | φ' } -> 
+    (sep_env Γ && sep_guards Ξ) |-- 
+      sep_pred (subst (subst_one ν x) φ) --> 
+      sep_pred (subst (subst_one ν x) φ').
+Proof.
+  intros.
+  inversion H1. subst.
+  simpl.
+  intro.
+  rewrite <- (subst_ty_prop φ (subst_one ν x) x0).
+  rewrite <- (subst_ty_prop φ' (subst_one ν x) x0).
+  apply derives_trans with
+    (Q := subst (subst_one ν x) (sep_env Γ) x0 &&
+          subst (subst_one ν x) (sep_guards Ξ) x0).
+  apply andp_derives.
+  apply vv_sub_env; assumption.
+  apply vv_sub_guards with (G := Γ); assumption.
+  unfold subst, Subst_pred, subst_pred.
+  simpl in H5.
+  apply H5.
+Qed.
+
+Lemma subtype_interp :
+  forall Γ Ξ φ φ' x b,
+    var_not_in ν Γ ->
+    wf_guards Γ Ξ ->
+    subtype Γ Ξ { ν : b | φ } { ν : b | φ' } -> 
+      sep_env Γ && sep_guards Ξ |-- 
+              sep_ty x { ν : b | φ } --> sep_ty x { ν : b | φ' }.
+Proof.
+  intros.
+  unfold sep_ty.
+  rewrite <- imp_andp_adjoint.
+  repeat apply andp_right.
+  apply andp_left2. apply andp_left1. apply andp_left1. apply derives_refl.
+  apply derives_trans with (Q := (sep_pred (subst (subst_one ν x) φ) 
+                              && (sep_pred (subst (subst_one ν x) φ) 
+                                 --> sep_pred (subst (subst_one ν x) φ')))).
+  apply andp_right.
+  apply andp_left2. apply andp_left1. apply andp_left2. apply derives_refl.
+  apply andp_left1. apply subtype_interp_pred with (b := b); assumption.
+  apply modus_ponens.
+  repeat apply andp_left1.
+  apply sep_env_pure.
+Qed.
+
+Lemma vv_sub_env_eval :
+  forall e ν x v w,
+    x <> ν -> 
+    eval w (subst (subst_one ν (var_e x)) e)
+    = eval (λ i : var, eval w (subst_one ν v i), hp w) (subst (subst_one ν (var_e x)) e).
+Proof.
+  induction e.
+  + intros. unfold subst, subst_one. reflexivity.
+  + intros. unfold subst, subst_one.
+    foo.
+  + intros. unfold subst, subst_one in *. 
+            unfold Subst_var_expr, subst_var, Language.subst_expr.
+            simpl in *.
+            unfold Subst_var_expr in *.
+            rewrite IHe1 with (v:=v).
+            rewrite IHe2 with (v:=v).
+            reflexivity.
+            assumption.
+            assumption.
+Qed.
+
+Lemma vv_sub_env_prop :
+  forall p ν x v w,
+    x <> ν ->
+    sep_pred (subst (subst_one ν (var_e x)) p) w =
+    sep_pred (subst (subst_one ν (var_e x)) p)
+             (λ i : var, eval w (subst_one ν v i), hp w).
+Proof.
+  intros.
+  induction p.
+  + constructor.
+  + destruct b. unfold subst, Subst_prop, subst_prop. simpl.
+    rewrite <- vv_sub_env_eval with (v := v).
+    rewrite <- vv_sub_env_eval with (v := v).
+    reflexivity.
+    assumption.
+    assumption.
+  + simpl in *. unfold subst in *. unfold imp.
+    rewrite IHp.
+    reflexivity.
+  + simpl. unfold subst, Subst_prop in *. 
+    unfold andp.
+    rewrite IHp1.
+    rewrite IHp2.
+    reflexivity.
+  + simpl. unfold subst, Subst_prop in *. 
+    unfold orp.
+    rewrite IHp1.
+    rewrite IHp2.
+    reflexivity.
+Qed.
+
+Lemma vv_sub_env_ty :
+  forall T x v,
+    x <> ν ->
+    sep_ty (var_e x) T |-- subst (subst_one ν v) (sep_ty (var_e x) T).
+Proof.
+  intros.
+  unfold sep_ty in *.
+  destruct T as [b p].
+  repeat rewrite subst_distr_andp.
+  repeat apply andp_derives.
+  unfold subst. 
+  unfold Subst_pred, subst_pred, subst_one.
+  unfold sep_base.
+  apply exp_left.
+  intro vv.
+  simpl.
+  intro w.
+  rewrite <- exp_andp1.
+  apply andp_derives.
+  apply prop_left.
+  intro EQ.
+  apply (exp_right vv).
+  apply prop_right.
+  destruct (eq_dec x ν). intuition. assumption.
+  trivial.
+  intro w.
+  rewrite vv_sub_env_prop with (v:= v).
+  apply derives_refl.
+  assumption.
+  trivial.
+Qed.
+
+Lemma subst_vv_env :
+  forall Γ,
+    var_not_in ν Γ ->
+    nonfreevars (sep_env Γ) ν.
+Proof.
+  intros.
+  induction Γ.
+  + unfold nonfreevars. intro. apply derives_refl.
+  + unfold sep_env. destruct a as [x [b p]].
+    fold sep_env.
+    unfold nonfreevars.
+    intro e.
+    repeat rewrite subst_distr_andp.
+    repeat apply andp_derives.
+    apply vv_sub_env_ty.
+      unfold var_not_in in H.
+      rewrite Forall_forall in H.
+      apply (H (x, { ν : b | p })); left; reflexivity.
+    apply IHΓ.
+    inversion H.
+    assumption.
+    trivial.
+Qed.
+
+Lemma sep_env_base_var :
+  forall Γ x b p,
+    (x, { ν : b | p }) ∈ Γ ->
+    sep_env Γ |-- sep_base (var_e x) b.
+Proof.
+  induction Γ.
+  + intros. inversion H.
+  + intros. 
+    apply in_inv in H. 
+    destruct a as [x' [b' p']].
+    destruct H.
+    inversion H. subst.
+    apply andp_left1.
+    apply andp_left1.
+    apply andp_left1.
+    apply andp_left1.
+    apply derives_refl.
+    unfold sep_env; fold sep_env.
+    apply andp_left1.
+    apply andp_left2.
+    apply (IHΓ _ _ p).
+    assumption.
+Qed.
+
+Lemma sep_env_base_val :
+  forall Γ (v : value),
+    sep_env Γ |-- sep_base v (base_of_val v).
+Proof.
+  intros.
+  unfold sep_base.
+  destruct (base_of_val v), v.
+  unfold base_of_type.
+  apply (exp_right n).
+  simpl. intro. apply andp_right. apply prop_right. reflexivity.
+  apply sep_env_pure.
+Qed.
+
+Lemma type_interp :
+  forall Γ Ξ x T,
+    var_not_in ν Γ ->
+    expr_type Γ Ξ x T ->
+    wf_guards Γ Ξ -> 
+    sep_env Γ && sep_guards Ξ |-- sep_ty x T.
+Proof.
+  intros Γ Ξ x T vvnotin ET. (* [ ν b φ ]  w SE ET. *)
+  unfold sep_ty.
+  dependent induction ET.
+  {
+    intros wfg.
+    apply andp_right.
+    apply andp_right.
+    apply andp_left1. 
+    apply sep_env_base_val.
+    intro w.
+    simpl.
+    apply andp_right.
+    apply prop_right.
+    unfold subst, Subst_var_expr, subst_one. simpl. foo.
+    apply andp_left1; apply sep_env_pure.
+    apply andp_left1; apply sep_env_pure.
+  }
+  {
+    intros wfg.
+    apply andp_right.
+    apply andp_right.
+  * apply andp_left1; apply sep_env_base_var with (p := φ); assumption.
+  * clear wfg.
+    apply andp_left1.
+    induction Γ.
+    + intuition.
+    + intros. 
+      destruct a as [x' [ b' p' ]].
+      apply in_inv in H.
+      destruct H.
+      inversion H; subst.
+      unfold sep_env; fold sep_env.
+      apply andp_left1.
+      apply andp_left1.
+      apply andp_left1.
+      apply andp_left2.
+      solve [intuition].
+      unfold sep_env; fold sep_env.
+      apply andp_left1.
+      apply andp_left2.
+      apply IHΓ.
+      inversion vvnotin. assumption.
+      assumption.
+   * apply andp_left1; apply sep_env_pure.
+  }
+  {
+    fold (sep_ty e T) in IHET.
+    fold (sep_ty e T').
+    intro.
+    apply derives_trans with (Q := sep_env Γ && sep_guards Ξ && sep_ty e T).
+    apply andp_right.
+    apply andp_right.
+      apply andp_left1; apply derives_refl.
+      apply andp_left2; apply derives_refl.
+      apply IHET; assumption.
+    apply imp_andp_adjoint.
+    destruct T, T'. inversion H0. subst.
+    apply subtype_interp; assumption.
+  }
+Qed.
+
+Lemma types_interp :
+  forall Γ Ξ xs ts,
+    var_not_in ν Γ ->  
+    wf_guards Γ Ξ ->
+    tc_list Γ Ξ (combine xs ts) ->
+    sep_env Γ && sep_guards Ξ |-- sep_env (combine xs ts).
+Proof.
+  intros.
+  unfold tc_list in H1.
+  rewrite Forall_forall in H1.
+  unfold sep_env.
+  induction (combine xs ts).
+  + normalize. apply andp_left1. apply sep_env_pure.
+  + destruct a. 
+    fold sep_env.
+    apply andp_right.
+    apply andp_right.
+    apply type_interp with (Γ := Γ);
+      [ assumption | apply H1 with (x := (v,r)); left; reflexivity | assumption].
+    apply IHl. 
+    intro. intro.
+    apply H1.
+    unfold In. right. apply H2.
+    apply andp_left1; apply sep_env_pure.
+Qed.
+
+Lemma funspec_nomem :
+  forall Φ p, 
+    fun_not_in p Φ ->
+    Forall (fun ps => fst4 ps <> p) (sep_proc_env Φ).
+Proof.
+  intros.
+  induction Φ.
+  + constructor.
+  + rewrite Forall_forall in *.
+    intros [ [[p' pr] P] Q ] mem.
+    destruct a as [p'' [s t]].
+    unfold sep_proc_env in mem. fold sep_proc_env in mem.
+    apply in_inv in mem.
+    destruct mem.
+    simpl in *.
+    unfold sep_schema in H0.
+    destruct t.
+    destruct s_ret.
+    inversion H0. subst.
+    unfold fun_not_in in H.
+    rewrite Forall_forall in H.
+    specialize (H (p', (s, {| s_formals := s_formals; s_formal_ts := s_formal_ts; s_ret := (v,r) |}))).
+    apply H.
+    left. reflexivity.
+    apply IHΦ.
+    inversion H. assumption.
+    assumption.
+Qed.
+    
+Lemma funspec_interp :
+  forall F f p t,
+    In (f, (p,t)) F -> In (sep_schema f p t) (sep_proc_env F).
+Proof.
+  intros.
+  induction F.
+  + inversion H.
+  + destruct H. destruct a. destruct p1. inversion H. subst.
+    apply in_inv. left. reflexivity.
+    apply IHF in H.
+    unfold sep_proc_env.
+    destruct a.
+    destruct p1.
+    simpl.
+    right.
+    apply H.
+Qed.
+(* Lemma sep_pred_pure : *)
+(*   forall p Q, *)
+(*     (sep_pred p && emp) && Q = sep_pred p * Q. *)
+(* Proof. *)
+(*   intros. *)
+(*   induction p. *)
+(*   simpl. *)
+(*   extensionality. *)
+(*   rewrite <- sepcon_emp at 1. *)
+(*   rewrite sepcon_comm. *)
+(*   apply pred_ext. *)
+(*   apply sepcon_derives. *)
+(*   apply prop_right. trivial. *)
+(*   apply andp_left2. apply derives_refl. *)
+  
+(*   unfold pure. *)
+(*   induction p. *)
+(*   simpl.  *)
+(*   repeat intro. *)
+(*   repeat (unfold join, Join_fun, Join_lower, Join_discrete in H0; hnf in H0). *)
+(*   destruct H0. *)
+(*   destruct a. destruct a0. destruct b. *)
+(*   unfold TT, prop in H. simpl in H. *)
+(*   unfold pure. *)
+
+(*   unfold identity. *)
+(*   hnf. *)
+(*   repeat intro. *)
+
+(*   unfold join in H0. *)
+(*   unfold Join_world in H0. *)
+(*   destruct a. *)
+(*   destruct a0. *)
+(*   destruct b.  *)
+(*   simpl in H0. *)
+(*   hnf in H0. *)
+(*   destruct H0. *)
+(*   simpl in *. *)
+(*   unfold join in *. *)
+(*   hnf in *. *)
+(*   unfold join, Join_equiv in *. *)
+(*   unfold join, Join_lower, Join_discrete in H1. *)
+(*   destruct H0 with (x := V 0). *)
+  
+
+Lemma sep_ty_pure_subst :
+  forall x t θ,
+    pure (subst θ (sep_ty x t)).
+Proof.
+  intros.
+  unfold pure.
+  destruct t.
+  unfold subst, sep_ty, Subst_pred, subst_pred.
+  intro w.
+  simpl.
+  apply andp_left2.
+  trivial.
+Qed.
+
+(* Lemma sep_env_pure : *)
+(*   forall G, *)
+(*     pure (sep_env G). *)
+(* Proof. *)
+(*   intros. *)
+(*   unfold pure. *)
+(*   intro. intro. *)
+(*   unfold identity. *)
+(*   intros w1 w2. *)
+(*   intros. *)
+(*   apply H0. *)
+(* Qed. *)
+
+(* Lemma sep_guards_pure : *)
+(*   forall G, *)
+(*     pure (sep_guards G). *)
+(* Proof. *)
+(*   unfold pure. *)
+(*   unfold identity. *)
+(*   intros. *)
+(*   intro. *)
+(*   intro. *)
+(*   intros w1 w2. *)
+(*   intro. *)
+(*   apply H0. *)
+(* Qed. *)
+
+Lemma sep_proof_skip :
+  forall Φ Ξ Γ Γ' (J : (Φ ; Γ ; Ξ) ⊢ skip_s ::: Γ'), 
+    sep_proc_env Φ |- {{ sep_env Γ * sep_guards Ξ }} skip_s {{ sep_env Γ' * sep_guards Ξ }}.
+Proof.
+  intros. inversion J. subst. constructor.
+Qed.
+
+Lemma sep_proof_assign :
+  forall Φ Ξ Γ Γ' x e (J : (Φ ; Γ ; Ξ)⊢ assign_s x e ::: Γ'), 
+    wf_env Γ ->
+    wf_guards Γ Ξ ->
+    sep_proc_env Φ |- {{ sep_env Γ * sep_guards Ξ }} assign_s x e {{ sep_env Γ' * sep_guards Ξ }}.
+Proof.
+  intros Φ Ξ Γ Γ' x e J wfenv wfguards.
+  inversion J. subst.
+  apply semax_frame.
+  apply semax_pre_post with (P' := (EX v : value, (eval_to e v))
+                                              && (subst_pred (subst_one x e )
+                                                             (sep_env ((x, {ν : τ | (var_e ν) .= e }) :: Γ))))
+                            (Q' := sep_env ((x,{ν : τ | (var_e ν) .= e }) :: Γ)).
+  apply andp_right.
+  unfold eval_to.
+  simpl.
+  intro w.
+  rewrite <- exp_andp1.
+  apply andp_right.
+  apply (expr_eval Γ Ξ e τ φ H7).
+  purity.
+  apply derives_trans with (Q := sep_env Γ && subst_pred (subst_one x e) (sep_env Γ)).
+  simpl. intro w.
+  rewrite subst_dom_env. 
+    apply andp_right; trivial.
+    assumption.
+    split. unfold subst_one. foo.
+    intros x' x'_in.
+    unfold subst_one. destruct (eq_dec x' x). subst.
+    unfold var_in, var_not_in in *.
+    rewrite Forall_forall in *.
+    destruct x'_in.
+    apply H5 in H.
+    contradiction H. reflexivity. reflexivity.
+    unfold subst_one. destruct (eq_dec ν x); congruence.
+  apply subst_env_eq_expr with (Grds := Ξ) (φ := φ).
+  assumption.
+  apply derives_refl.
+  rewrite exp_andp1.
+  apply semax_assign with (e := e) (x := x) (P := (sep_env ((x, {ν : τ | var_e ν .= e}) :: Γ))).
+  unfold subset.
+  intros.
+  inversion H. subst.
+  apply wf_guards_nonfree with (Γ := Γ); assumption.
+Qed.
+
+Lemma sep_args_sub :
+  forall Γ Ξ (xs' : list var) ts' (θ : subst_t var var) xs ts,
+    length xs = length ts ->
+    xs' = subst θ xs ->
+    ts' = subst θ ts ->
+    tc_list Γ Ξ (combine xs' ts') ->
+    var_not_in ν Γ -> 
+    wf_guards Γ Ξ ->
+    sep_env Γ && sep_guards Ξ |-- sep_env (subst θ (combine xs ts)).
+Proof.
+  intros.
+  assert (C: subst θ (combine xs ts) =
+                      combine xs' ts').
+    rewrite H0. rewrite H1.
+    rewrite <- subst_combine with (xs := xs) (ys := ts).
+    reflexivity.
+    assumption.
+  rewrite C.
+  apply types_interp; assumption.
+Qed.
+
+Lemma sep_env_cons :
+  forall x t Γ,
+    sep_ty (var_e x) t * sep_env Γ |-- sep_env ((x,t) :: Γ).
+Proof.
+  intros.
+  unfold sep_env at 2. fold sep_env.
+  rewrite <- sepcon_emp at 1.
+  rewrite <- sepcon_pure_andp.
+  rewrite <- sepcon_pure_andp.
+  apply sepcon_derives.
+  apply sepcon_derives.
+  apply derives_refl.
+  apply derives_refl.
+  apply derives_refl.
+  apply sep_ty_pure.
+  apply sep_env_pure.
+  unfold pure. apply andp_left1. apply sep_ty_pure.
+  apply derives_refl.
+Qed.
+  
+Lemma sep_env_cons_sub :
+  forall x b p θ Γ,
+    θ ν = ν -> (forall x , θ x = ν -> x = ν) ->
+    subst θ (sep_ty (var_e x) { ν : b | p }) * sep_env Γ
+    |-- sep_env ((subst θ (x,{ ν : b | p })) :: Γ).
+Proof.
+  intros x b p θ Γ vv_id vv_im.
+  unfold sep_env; fold sep_env.
+  rewrite sepcon_pure_andp.
+  simpl.
+  intro w.
+  apply andp_right.
+  apply andp_derives.
+  rewrite subst_lift_assert.
+  rewrite <- subst_ty_distr. 
+  unfold sep_ty. simpl.
+  apply andp_derives.
+  apply andp_derives.
+  unfold subst, Subst_var_var. apply derives_refl.
+  unfold subst. simpl.
+  rewrite subst_lift_pred. unfold subst. simpl. apply derives_refl.
+  apply derives_refl.
+  rewrite vv_id. reflexivity.
+  apply subst_vv_not_in_range.
+  intro v. split. apply vv_im. intro. rewrite H. assumption.
+  apply derives_refl.
+  apply andp_left2. apply sep_env_pure.
+  apply sep_ty_pure_subst.
+  apply sep_env_pure.
+Qed.
+
+Lemma sep_proof_proc_ret :
+  forall (θ : subst_t var var) x t Γ, 
+    θ ν = ν -> (forall x, θ x = ν -> x = ν) ->
+    wf_type (subst θ (x,t) :: Γ) (subst θ t)  ->
+   (subst θ (sep_ty (var_e x) t)) * sep_env Γ |--
+    sep_env ((subst θ (x,t)) :: Γ).
+Proof.
+  intros θ x t Γ vvid vvim wf H.
+  destruct t as [ b p ].
+  simpl in *.
+  apply sep_env_cons_sub. 
+  assumption.
+  assumption.
+Qed.
+
+Lemma sep_proof_proc_sub :
+  forall x v θ,
+    v  = subst θ x ->
+    (forall x', θ x' = v <-> x = x') ->
+    unique_sub θ x.
+Proof.
+  intros x v θ vdef subprop.
+  unfold unique_sub.
+  exists v.
+  split.
+  symmetry. apply vdef.
+  intros.
+  unfold not_free_in.
+  specialize (subprop x0).
+  destruct subprop.
+  intuition.
+  apply H.
+  symmetry.
+  intuition.
+Qed.
+
+Lemma sep_proof_proc_mod :
+  forall f xs x x',
+    modvars (proc_s f xs x []) x' -> x = x'.
+Proof.
+  intros.
+  inversion H.
+  intuition.
+  reflexivity.
+Qed.
+
+Ltac wfenv_ty_t :=
+  match goal with 
+    | [ X : ?x = ?a, Y : ?y = ?b, H : wf_type _ _ |- _ ] =>
+      rewrite X in H; rewrite Y in H; assumption
+    | [ H : (?x, ?y) = subst _ (_, _) |- _ ] => 
+      unfold subst, Subst_prod, subst_prod in H; inversion H; wfenv_ty_t
+    | [ H : wf_env (subst ?x (?f ?z) :: ?G) |- wf_type (subst ?x (?f ?z) :: ?G) _ ]  =>
+      inversion H; destruct (f z); simpl in *; wfenv_ty_t
+  end.
+
+Lemma lift_assert :
+  forall {P Q : assert} w, P |-- Q ->(P w |-- Q w).
+Proof.
+  intros.
+  apply H.
+Qed.
+
+Lemma sep_proof_proccall :
+  forall Φ Ξ Γ Γ' f xs v (J : (Φ ; Γ ; Ξ) ⊢ proc_s f xs v [] ::: Γ'),
+    wf_env Γ ->
+    wf_guards Γ Ξ ->
+    sep_proc_env Φ |- {{ sep_env Γ * sep_guards Ξ }} proc_s f xs v [] {{ sep_env Γ' * sep_guards Ξ }}.
+Proof.
+  intros until v. 
+  intros J wf wfg.
+  inversion J as [ | ? ? ? ? ? p S ? ? θ θS fmem wfS wfθ 
+                     ? ? ? ? retid substid wfenv wfsubty tclist
+                     | | | ]. 
+  simpl in *. subst.
+  destruct S as [fxs fts [rx rt]] eqn:S_def.
+  simpl in *.
+  apply funspec_interp in fmem.
+  unfold sep_schema in fmem. 
+  apply semax_pre_post with 
+  (P' := ((Subst.subst θ (sep_env (combine fxs fts)))) * (sep_env Γ * sep_guards Ξ)) 
+  (Q' := ((Subst.subst θ (sep_ty (var_e rx) rt))) * (sep_env Γ * sep_guards Ξ)).
+  intro w.
+  simpl.
+  rewrite <- (subst_in_env Γ).
+  rewrite sepcon_pure_andp at 1.
+2: purity.
+2: purity.
+  rewrite (sepcon_pure_andp (sep_env (subst θ (combine fxs fts)) w)). 
+2: purity.
+2: purity.
+  apply andp_right.
+  pose sep_args_sub as argstc; simpl in argstc; apply argstc with (xs' := subst θ fxs) (ts' := subst θ fts).
+  inversion wfS; assumption.
+  reflexivity.
+  reflexivity.
+  assumption.
+  apply wf_env_no_vv; assumption.
+  assumption.
+  rewrite sepcon_pure_andp; try apply derives_refl; purity.
+  wfsubst θ.
+  assumption.
+  assumption.
+  rewrite subst_combine.
+  apply forall_p_combine.
+  inversion wfS; repeat rewrite <- subst_length; assumption.
+  assumption.
+  inversion wfS; assumption.
+  rewrite <- sepcon_assoc.
+  simpl.
+  intro w.
+  apply sepcon_derives.
+  pose sep_proof_proc_ret as RT; simpl in RT; apply RT.
+  apply wfθ; reflexivity.
+  apply wfθ.
+  inversion wfenv; assumption.
+  apply derives_refl.
+  apply semax_frame.
+  subst.
+  assert (A : subst θ (proc_s f fxs rx []) = proc_s f (subst θ fxs) (subst θ rx) []).
+  unfold subst at 1. simpl. reflexivity.
+  rewrite <- A.
+  apply semax_subst.
+  apply (semax_proc f (mkProc fxs rx [] p)).
+  assumption.
+  intros.
+  assert (rx = x) by 
+      (apply sep_proof_proc_mod with (f:=f) (xs:= fxs); assumption).
+  subst.
+  apply sep_proof_proc_sub with (v := subst θ x).
+  reflexivity.
+  intros.
+  specialize (retid x').
+  constructor; intro; [ symmetry | idtac ]; apply retid; [ idtac | symmetry]; assumption.
+  unfold subset.
+  intros.
+  unfold nonfreevars.
+  intros.
+  assert (A : subst θ rx = x).
+    apply sep_proof_proc_mod with (f := f) (xs := subst θ fxs).
+    assumption.
+  assert (B : x <> ν).
+    inversion wfenv.
+    rewrite <- A.
+    assumption.
+  rewrite sepcon_pure_andp.
+2: purity.
+2: purity.
+  rewrite subst_distr_andp.
+  apply andp_derives.
+  simpl.
+  unfold subst, Subst_pred.
+  intro w.
+  rewrite subst_dom_env.
+    apply derives_refl.
+    assumption.
+    apply subst_one_is_disj.
+    assumption.
+    assumption.
+    inversion wfenv. rewrite <- A. assumption.
+    unfold subst_one. foo.
+  intro w.
+  rewrite subst_dom_guards with (Γ := Γ).
+  apply derives_refl.
+  assumption.
+  apply subst_one_is_disj.
+  assumption.
+  assumption.
+  inversion wfenv. rewrite <- A. assumption.
+Qed.
+
+Lemma subtype_same_base :
+  forall Ξ Γ b b' p p',
+    subtype Γ Ξ { ν : b | p } { ν : b' | p' } ->
+    subtype Γ Ξ { ν : b | p } { ν : b | p' }.
+Proof.
+  intros.
+  inversion H.
+  subst.
+  assumption.
+Qed.
+
+Lemma types_interp2 :
+  forall Ξ Γ Γ', 
+    wf_env Γ -> wf_guards Γ Ξ ->
+   (forall x t, (x,t) ∈ Γ' -> (exists t1, (x,t1) ∈ Γ /\ subtype Γ Ξ t1 t)) ->
+   sep_env Γ && sep_guards Ξ |-- sep_env Γ'.
+Proof.
+  intros Ξ Γ Γ' wfe wfg H.
+  induction Γ' as [| [x t]].
+  + apply andp_right. normalize. purity.
+  + unfold sep_env; fold sep_env.
+    apply andp_right.
+    apply andp_right.
+    specialize (H x t).
+    destruct H. left. reflexivity.
+    destruct t as [b p].
+    destruct x0 as [b0 p0].
+    apply derives_trans with (Q := sep_env Γ && sep_guards Ξ && sep_ty (var_e x) {ν : b | p0}).
+    apply andp_right. trivial. apply type_interp.
+    apply wf_env_no_vv.
+    exact wfe.
+    constructor.
+    destruct H. inversion H0. subst.
+    apply H.
+    exact wfg.
+    rewrite imp_andp_adjoint.
+    pose subtype_interp as ST. simpl in ST. simpl. apply ST.
+    apply wf_env_no_vv.
+    exact wfe.
+    exact wfg.
+    destruct H.
+    inversion H0; subst.
+    assumption.
+    apply IHΓ'.
+    intros x0 t0 x0mem.
+    apply H.
+    right.
+    apply x0mem.
+    purity.
+Qed.
+
+Lemma join_swap :
+  forall Γ1 Γ2 Γ' Ξ,
+    join_env Ξ Γ1 Γ2 Γ' <-> join_env Ξ Γ2 Γ1 Γ'.
+Proof.
+  intros.
+  unfold join_env.
+  constructor.
+  intros [a [b c]].
+  split.
+  assumption.
+  split.
+  intros xt.
+  specialize (b xt).
+  rewrite and_comm.
+  apply b.
+  unfold join_var in *.
+  rewrite Forall_forall in *.
+  intros [x t].
+  intro.
+  destruct c with (x,t).
+  apply H.
+  split.
+  apply H0.
+  rewrite and_comm.
+  apply H1.
+  intros [a [b c]].
+  split.
+  assumption.
+  split.
+  intros xt.
+  specialize (b xt).
+  rewrite and_comm.
+  apply b.
+  unfold join_var in *.
+  rewrite Forall_forall in *.
+  intros [x t].
+  intro.
+  destruct c with (x,t).
+  apply H.
+  split.
+  apply H0.
+  rewrite and_comm.
+  apply H1.
+Qed.
+  
+Lemma join_interp :
+  forall Γ1 Γ2 Γ' Ξ ,
+    wf_env Γ1 -> wf_env Γ2 -> wf_guards Γ1 Ξ ->
+    join_env Ξ Γ1 Γ2 Γ' ->
+    (sep_env Γ1 && sep_guards Ξ) |-- sep_env Γ' && sep_guards Ξ.
+Proof.
+  intros until Ξ.
+  intros wf1 wf2 wfg J.
+  apply andp_right.
+  destruct J as [wfJ [J1 J2]].
+  rewrite Forall_forall in J2.
+  unfold join_var in J2.
+  apply types_interp2.
+  assumption.
+  assumption.
+  intros x t xtmem.
+  specialize (J2 (x,t) xtmem).
+  apply J2.
+  apply andp_left2; apply derives_refl.
+Qed.
+
+Lemma sep_proof_if_derives :
+  forall Ξ Γ Γ1 Γ2 Γ' e t g,
+    wf_env Γ ->
+    wf_env Γ1 ->
+    wf_env Γ2 ->
+    wf_guards Γ Ξ ->
+    wf_guards Γ1 Ξ ->
+    wf_guards Γ2 Ξ ->
+    join_env Ξ Γ1 Γ2 Γ' ->
+    expr_type Γ Ξ e t ->
+    (* (Φ; Γ; not_r (e .= int_v 0) :: Ξ)⊢s1 ::: (Γ1) -> *)
+    (* (Φ; Γ; (e .= int_v 0) :: Ξ)⊢s2 ::: (Γ2) -> *)
+    sep_env Γ1 * sep_guards (g :: Ξ) |-- sep_env Γ' && sep_guards Ξ.
+Proof.
+  intros until g. intros wf wf1 wf2 wfg wfg1 wfg2 joinenv et.
+  unfold sep_guards; fold sep_guards.
+  rewrite sepcon_pure_andp.
+2: purity.
+2: purity.
+  repeat rewrite <- andp_assoc.
+  apply andp_left1.
+  rewrite andp_assoc.
+  rewrite andp_comm.
+  rewrite andp_assoc.
+  apply andp_left2.
+  rewrite andp_comm.
+  apply join_interp with (Γ2 := Γ2); assumption.
+Qed.
+
+Lemma wf_guard_expr_type1 :
+  forall Γ Ξ e t,
+    wf_env Γ ->
+    expr_type Γ Ξ e t ->
+    wf_guard Γ (e .= int_v 1).
+Proof.
+  intros.
+  split.
+  repeat constructor.
+  apply wf_expr_ty_expr with Ξ t.
+    assumption.
+  simpl. rewrite  app_nil_r.
+  apply wf_expr_ty_expr_fv with Γ Ξ t; assumption.
+Qed.
+
+Lemma wf_guard_expr_type2 :
+  forall Γ Ξ e t,
+    wf_env Γ ->
+    expr_type Γ Ξ e t ->
+    wf_guard Γ (e .= int_v 0).
+Proof.
+  intros.
+  split.
+  repeat constructor.
+  apply wf_expr_ty_expr with Ξ t.
+    assumption.
+  simpl. rewrite  app_nil_r.
+  apply wf_expr_ty_expr_fv with Γ Ξ t; assumption.
+Qed.
+
+Lemma sep_proof_if :
+  forall Φ Ξ Γ Γ1 Γ2 Γ' s1 s2 e t,
+    wf_env Γ ->
+    wf_guards Γ Ξ ->
+    expr_type Γ Ξ e t ->
+    (Φ; Γ; (e .= int_v 1) :: Ξ)⊢s1 ::: (Γ1) ->
+    (Φ; Γ; (e .= int_v 0) :: Ξ)⊢s2 ::: (Γ2) ->
+    join_env Ξ Γ1 Γ2 Γ' ->
+    (wf_env Γ
+         → wf_guards Γ ((e .= int_v 1) :: Ξ)
+           → sep_proc_env Φ |- 
+             {{sep_env Γ * sep_guards ((e .= int_v 1) :: Ξ)}}s1
+             {{sep_env Γ1 * sep_guards ((e .= int_v 1) :: Ξ)}}) ->
+    (wf_env Γ
+       → wf_guards Γ ((e .= int_v 0) :: Ξ)
+         → sep_proc_env Φ |- 
+           {{sep_env Γ * sep_guards ((e .= int_v 0) :: Ξ)}}s2
+           {{sep_env Γ2 * sep_guards ((e .= int_v 0) :: Ξ)}}) ->
+    sep_proc_env Φ |- {{ sep_env Γ && sep_guards Ξ }} 
+                        if_s e s1 s2 
+                        {{ sep_env Γ' && sep_guards Ξ }}.
+Proof.
+  intros until t.
+  intros wf wfg et H1 H2 joinenv IH1 IH2.
+  assert (WF1 : wf_env Γ1).
+    apply wf_env_stmt with Φ Γ ((e .= int_v 1) :: Ξ) s1; assumption.
+  assert (WF2 : wf_env Γ2).
+    apply wf_env_stmt with Φ Γ (((e .= int_v 0)) :: Ξ) s2; assumption.
+  assert (WFG1 : wf_guards Γ1 ((e .= int_v 1) :: Ξ)).
+    apply wf_guards_stmt with Φ Γ s1. assumption. assumption.
+    apply Forall_cons. 
+      apply wf_guard_expr_type1 with Ξ t; assumption. 
+      assumption.
+  assert (WFG2 : wf_guards Γ2 ((e .= int_v 0) :: Ξ)).
+    apply wf_guards_stmt with Φ Γ s2. assumption. assumption.
+    apply Forall_cons. 
+      apply wf_guard_expr_type2 with Ξ t; assumption. 
+      assumption.
+  apply semax_if.
+  rewrite andp_comm.
+  rewrite andp_assoc.
+  rewrite andp_comm with (P := sep_guards Ξ).
+  apply semax_pre_post with (P' := sep_env Γ * sep_guards ((e .= int_v 1) :: Ξ))
+                            (Q' := sep_env Γ1 * sep_guards ((e .= int_v 1) :: Ξ)).
+  rewrite sepcon_pure_andp.
+    repeat apply andp_right.
+    apply andp_left1. apply derives_refl.
+    apply andp_left2. apply andp_left1. 
+    unfold eval_to. simpl. intro. apply andp_left1. apply derives_refl.
+    apply andp_left1. purity.
+    fold sep_guards.
+    do 2 apply andp_left2. apply derives_refl.
+    apply andp_left1. purity.
+    purity.
+    apply sep_guard_pure.
+  apply sep_proof_if_derives with Γ Γ2 e t.  
+    assumption.
+    assumption.
+    assumption.
+    assumption.
+    inversion WFG1; assumption.
+    inversion WFG2; assumption.
+    assumption.
+    assumption.
+  apply IH1.
+  assumption.
+  apply Forall_cons.
+    apply wf_guard_expr_type1 with Ξ t; assumption.
+    assumption.
+  apply semax_pre_post with (P' := sep_env Γ * sep_guards ((e .= int_v 0) :: Ξ))
+                            (Q' := sep_env Γ2 * sep_guards ((e .= int_v 0) :: Ξ)).
+    rewrite sepcon_pure_andp.
+    repeat apply andp_right.
+    apply andp_left2. apply andp_left1. apply derives_refl.
+    apply andp_left1. unfold eval_to. intro. apply andp_left1. apply derives_refl.
+    apply andp_left2. purity.
+    fold sep_guards.
+    apply andp_left2. apply andp_left2. apply derives_refl.
+    apply andp_left2. purity.
+    purity.
+    apply sep_guard_pure.
+  apply sep_proof_if_derives with Γ Γ1 e t;
+    repeat first [ assumption | inversion WFG1; assumption | inversion WFG2; assumption].
+  apply join_swap. assumption.
+  apply IH2.
+  assumption.
+  apply Forall_cons.
+    apply wf_guard_expr_type2 with Ξ t; assumption.
+    assumption.
+Qed.
+
+Theorem sep_proof_stmt :
+  forall Φ Ξ Γ Γ' s (J : (Φ ; Γ ; Ξ) ⊢ s ::: Γ'),
+    wf_env Γ ->
+    wf_guards Γ Ξ ->
+    sep_proc_env Φ |- {{ sep_env Γ && sep_guards Ξ }} s {{ sep_env Γ' && sep_guards Ξ }}.
+Proof.
+  intros.
+  rewrite <- sepcon_pure_andp.
+  rewrite <- sepcon_pure_andp.
+  dependent induction J.
+  + apply sep_proof_skip with (Φ := Φ) (Ξ := Ξ). constructor.
+  + apply sep_proof_proccall with (Φ := Φ) (Ξ := Ξ).
+    econstructor; eauto.
+    assumption.
+    assumption.
+  + apply sep_proof_assign with (Φ := Φ) (Ξ := Ξ). 
+    econstructor; eauto.
+    assumption.
+    assumption.
+  + repeat rewrite sepcon_pure_andp.
+    apply sep_proof_if with Γ1 Γ2 { ν : int_t | p }; assumption.
+    purity.
+    purity.
+    purity.
+    purity.
+  + apply semax_seq with (Q := sep_env Γ' * sep_guards Ξ).
+    apply IHJ1; assumption.
+    apply IHJ2. 
+    apply wf_env_stmt with (P := Φ) (G := Γ) (X := Ξ) (s := s1); assumption.
+    apply wf_guards_stmt with (P := Φ) (G := Γ) (X := Ξ) (s := s1); assumption.
+ + apply sep_env_pure.
+ + apply sep_guard_pure.
+ + apply sep_env_pure.
+ + apply sep_guard_pure.
+Qed.
+
+Corollary type_safety_stmt :
+  forall Φ Γ s, (Φ ; [] ; []) ⊢ s ::: Γ -> sep_proc_env Φ |- {{ emp }} s {{ TT }}.
+Proof.
+  intros.
+  assert (wf_env nil). constructor.
+  assert (wf_guards nil nil). constructor.
+  apply semax_pre_post with (P' := sep_env nil && sep_guards nil) 
+                            (Q' := sep_env Γ && sep_guards nil);
+  first [ apply sep_proof_stmt with (Φ := Φ) (Ξ := []); assumption
+        | unfold sep_guards; normalize ].
+Qed.
+
+Theorem sep_proof_program :
+  forall Φ p,
+    prog_type Φ p -> semax_prog (sep_proc_env Φ) p.
+Proof.
+  intros Φ p H.
+  induction H.
+  + constructor.
+    apply type_safety_stmt with Γ; assumption.
+  + assert (WFΓ : wf_env Γ).
+      inversion H.
+      pose (wf_env_stmt _ _ Γ _ body H9 H5).
+      apply w.
+    destruct pr. 
+    simpl in *.
+    subst.
+    pose (@semax_procdecl_p (sep_proc_env Φ)
+                           e
+                           body
+                           (sep_schema p (seq_s body (return_s e)) S)
+                           prog) as P.
+    unfold sep_schema in P.
+    destruct S.
+    destruct s_ret.
+    simpl in *.
+    simpl in *.
+    apply P.
+    reflexivity.
+    apply funspec_nomem.
+    assumption.
+    simpl in *.
+    apply semax_pre_post with (P' := sep_env (combine s_formals s_formal_ts) && sep_guards [])
+                              (Q' := sep_env Γ && sep_guards []).
+    apply andp_right. 
+      apply derives_refl. 
+      unfold sep_guards. apply andp_right. normalize. purity.
+    destruct r as [ τ φ ].
+    apply derives_trans with (Q := sep_ty (subst (subst_one v e) (var_e v)) 
+                                         (subst (subst_one v e) {ν : τ | φ})).
+    unfold subst, Subst_var_expr, subst_one at 1, Language.subst_expr.
+    destruct (eq_dec v v).
+    apply type_interp.
+    inversion H.
+    apply wf_env_no_vv. 
+    apply WFΓ.
+    assumption.
+    constructor.
+    intuition.
+    intro.
+    rewrite subst_ty_distr. apply derives_refl.
+    inversion H.
+    clear P. clear H1.
+    inversion H3.
+    unfold subst_one.
+    destruct (eq_dec ν v). intuition. subst. reflexivity.
+    assert (NEQ : v <> ν).
+    inversion H.
+    inversion H3. assumption.
+    apply subst_vv_not_in_range_exp.
+    apply wf_expr_ty_expr_fv with (Γ := Γ) (Ξ := []) (T := subst (subst_one v e) { ν : τ | φ }).
+    apply WFΓ.
+    assumption.
+    apply sep_proof_stmt in H5.
+    apply H5.
+    inversion H.
+    apply H2.
+    constructor.
+    apply IHprog_type.
 Qed.
